update heap definition
our current heap definition is a partial map that does not preserve
freed cells. This is gonna be problematic later on when we want to
prove the heap manipulation proof rules.

This changes the underlying value in the map from a value to a
disjoint union of a value or a Reserved cell.

Reserved is a value that only the EFree expression can put in the
heap and it is used to distinguish cells that were previously allocated
and freed from cells that were never allocated.

The head_step rule for EAlloc then changes to allow not only
allocating unused cells but the Reserved too. The head_step rule
for EFree, EStore, ELoad instead change the lookup value to be
Some (Value w) because we have to restric us from loading previously
deallocated cells.

The Alloc_head_step rule could be split into two, one for each result of
lookup that we allow, None and Some (Reserved) but this can be
unified using another predicate.

m !! l = Some e -> e = Reserved gives us both the allowed cases;
if location l has value e then it is a Reserve, meaning that it
was previously freed.

lang.v
@@ -113,7 +113,15 @@ Fixpoint subst (x : string) (w : val) (e : expr) : expr :=
   | EError => EError
   end.
 
-Notation mem := (gmap nat val).
+Inductive either :=
+| Value: val -> either
+| Reserved : either
+.
+
+Notation mem := (gmap nat either).
+
+(* a valid allocation cell is one where there is no current Value *)
+Definition valid_alloc (m : mem) (l : nat) := ∀ e, m !! l = Some e → e = Reserved.  
 
 Definition memfresh (m : mem) : nat := fresh (dom (gset nat) m).
 
@@ -140,17 +148,17 @@ Inductive head_step : expr → mem → expr → mem → Prop :=
      eval_bin_op op v1 v2 = Some v →
      head_step (EOp op (EVal v1) (EVal v2)) m (EVal v) m
   | Alloc_headstep m v l:
-     lookup l m = None →
-     head_step (EAlloc (EVal v)) m (EVal (VLoc l)) (insert l v m)
-  | Free_headstep m l :
-     lookup l m <> None →
-     head_step (EFree (EVal (VLoc l))) m (EVal VUnit) (delete l m)
+     valid_alloc m l →
+     head_step (EAlloc (EVal v)) m (EVal (VLoc l)) (<[ l := (Value v) ]> m)
+  | Free_headstep m l v:
+     m !! l = (Some (Value v)) →
+     head_step (EFree (EVal (VLoc l))) m (EVal VUnit) (<[l := Reserved ]> m)
   | Load_headstep m l v :
-     lookup l m = (Some v) →
+     m !! l = (Some (Value v)) →
      head_step (ELoad (EVal (VLoc l))) m (EVal v) m
-  | Store_headstep m l v :
-     lookup l m <> None →
-     head_step (EStore (EVal (VLoc l)) (EVal v)) m (EVal VUnit) (<[ l := v ]> m)
+  | Store_headstep m l v w:
+     m !! l = (Some (Value w)) →
+     head_step (EStore (EVal (VLoc l)) (EVal v)) m (EVal VUnit) (<[ l := (Value v) ]> m)
   (* new : the ambiguos expression reduces to any natural number *)
   | Amb_headstep m (n : nat):
      head_step EAmb m (EVal (VNat n)) m.
@@ -164,12 +172,15 @@ Inductive head_step : expr → mem → expr → mem → Prop :=
 
 Lemma Alloc_fresh_headstep m l v:
       l = (memfresh m) →
-      head_step (EAlloc (EVal v)) m (EVal (VLoc l)) (insert l v m).
+      head_step (EAlloc (EVal v)) m (EVal (VLoc l)) (<[ l := (Value v)]> m).
 Proof.
   intros ->.
   econstructor.
-  apply memfresh_is_fresh.
-  Qed.
+  unfold valid_alloc.
+  intros e H.
+  rewrite memfresh_is_fresh in H.
+  discriminate.
+Qed.
 
 Create HintDb head_step.
 Hint Constructors head_step : head_step.
@@ -288,8 +299,9 @@ Qed.
 (* later on we can define is_error as an expression that does not step anymore
    and to actually get to prove errors about resources we need some lemmas
    to discharge this to assumptions on the heaps *)
+
 Lemma step_alloc v l m:
-  step (EAlloc (EVal v)) m (EVal (VLoc l)) (<[l:=v]> m) ↔ m !! l = None.
+  step (EAlloc (EVal v)) m (EVal (VLoc l)) (<[l:= (Value v)]> m) ↔ valid_alloc m l.
 Proof.
   split.
   - intro.
@@ -300,38 +312,34 @@ Proof.
       assumption.
     + simpl in *.
       destruct c; simpl in *; discriminate.
-  - intro.
+  - intro H.
     change (EAlloc (EVal v)) with (fill []  (EAlloc (EVal v))).
     change (EVal (VLoc l)) with (fill [] (EVal (VLoc l))).
     econstructor.
-    constructor.
+    econstructor.
     assumption.
 Qed.
 
 Lemma step_alloc_inv e v m m':
-  step (EAlloc (EVal v)) m e m' ↔ ∃ l, e = (EVal (VLoc l)) ∧ m !! l = None ∧ m' = <[l:=v]> m.
+  step (EAlloc (EVal v)) m e m' ↔ ∃ l, e = (EVal (VLoc l)) ∧ valid_alloc m l ∧ m' = <[l := (Value v)]> m.
 Proof.
   split; intro.
   - inversion H.
     destruct E.
     + simpl in *; subst.
-      inversion H1.
-      exists l.
-      split; auto.
+      inversion H1; exists l; do 2 split; auto; rewrite H2; intro; discriminate.
     + destruct c; simpl in *; discriminate || auto.
-      * inversion H0.
-        destruct E; simpl in *.
-        subst e1.
-        inversion H1.
-        destruct c; simpl in *; discriminate.
+      * inversion H0; destruct E; simpl in *.
+        -- subst e1. inversion H1.
+        -- destruct c; simpl in *; discriminate.
   - destruct H as (loc & value & precondition & final_heap).
     subst.
     apply step_single.
-    auto using head_step.
+    eauto using head_step.
 Qed.
 
 Lemma step_free l m:
- step (EFree (EVal (VLoc l))) m (EVal VUnit) (delete l m) ↔   m !! l ≠ None.
+ step (EFree (EVal (VLoc l))) m (EVal VUnit) (<[l := Reserved ]> m) ↔ ∃ v, m !! l = (Some (Value v)).
 Proof.
   split.
   - intro.
@@ -339,19 +347,20 @@ Proof.
     destruct E.
     + rewrite fill_empty_context in *; subst.
       inversion H3.
-      assumption.
+      exists v; assumption.
     + simpl in *.
       destruct c; simpl in *; discriminate.
   - intro.
+    destruct H as [v H].
     change (EFree (EVal (VLoc l))) with (fill [] (EFree (EVal (VLoc l)))).
     change (EVal VUnit) with (fill [] (EVal VUnit)).
     econstructor.
-    constructor.
-    assumption.
+    econstructor.
+    eassumption.
 Qed.
 
 Lemma step_free_inv e l m m':
-  step (EFree (EVal (VLoc l))) m e m' ↔ e = (EVal VUnit) ∧ m !! l ≠ None ∧ m' = delete l m.
+  step (EFree (EVal (VLoc l))) m e m' ↔ ∃ v, e = (EVal VUnit) ∧ m !! l = (Some (Value v)) ∧ m' = <[ l := Reserved ]> m.
 Proof.
   split.
   - intro.
@@ -359,6 +368,7 @@ Proof.
     destruct E; simpl in *.
     + subst.
       inversion H1.
+      exists v.
       split; auto.
     + destruct c; simpl in *; discriminate || auto.
       * inversion H0.
@@ -366,12 +376,13 @@ Proof.
         subst.
         inversion H1.
         destruct c; simpl in *; discriminate || auto.
-  - intros [-> [Hlookup ->]].
+  - intros [v [-> [Hlookup ->]]].
     apply step_free; auto.
+    eauto.
 Qed.
 
 Lemma step_load l v m:
-  step (ELoad (EVal (VLoc l))) m (EVal v) m ↔  m !! l = Some(v).
+  step (ELoad (EVal (VLoc l))) m (EVal v) m ↔  m !! l = Some (Value v).
 Proof.
   split.
   - intro.
@@ -388,11 +399,10 @@ Proof.
     econstructor.
     constructor.
     assumption.
-
 Qed.
 
 Lemma step_load_inv e l m m':
-  step (ELoad (EVal (VLoc l))) m e m' ↔ ∃ v, e = (EVal v) ∧ m !! l = Some(v) ∧ m' = m.
+  step (ELoad (EVal (VLoc l))) m e m' ↔ ∃ v, e = (EVal v) ∧ m !! l = (Some (Value v)) ∧ m' = m.
 Proof.
   split.
   - intro.
@@ -410,7 +420,7 @@ Proof.
 Qed.
 
 Lemma step_store l v m:
-  step (EStore (EVal (VLoc l)) (EVal v)) m (EVal VUnit) (<[l:=v]> m) ↔ m !! l ≠ None.
+  step (EStore (EVal (VLoc l)) (EVal v)) m (EVal VUnit) (<[l:= (Value v)]> m) ↔ ∃ w, m !! l = Some (Value w).
 Proof.
   split.
   - intro.
@@ -418,25 +428,28 @@ Proof.
     destruct E.
     + rewrite fill_empty_context in *; subst.
       inversion H3.
-      assumption.
+      eauto.
     + simpl in *.
       destruct c; simpl in *; discriminate || auto.
   - intro.
+    destruct H as [w H].
     change (EStore (EVal (VLoc l)) (EVal v)) with (fill [] (EStore (EVal (VLoc l)) (EVal v))).
     change (EVal VUnit) with (fill [] (EVal VUnit)).
     econstructor.
     econstructor.
-    assumption.
+    eauto.
 Qed.
 
 Lemma step_store_inv l v e m m':
-  step (EStore (EVal (VLoc l)) (EVal v)) m e m' ↔ m !! l ≠ None ∧ e = (EVal VUnit) ∧ m' = (<[l:=v]> m).
+  step (EStore (EVal (VLoc l)) (EVal v)) m e m' ↔ ∃ w, m !! l = (Some (Value w)) ∧ e = (EVal VUnit) ∧ m' = (<[l:= (Value v)]> m).
 Proof.
    split.
   - intro.
     inversion H.
     destruct E; simpl in *; discriminate || auto; subst.
     + inversion H1; simpl in *; discriminate || auto; subst.
+      exists w.
+      split; auto.
     + destruct c; simpl in *; discriminate || auto; subst.
       * inversion H0.
         destruct E; simpl in *; discriminate || auto; subst.
@@ -446,8 +459,9 @@ Proof.
         destruct E; simpl in *; discriminate || auto; subst.
         inversion H1.
         destruct c; simpl in *; discriminate || auto.
-  - intros [Hlookup [->  ->]].
+  - intros [w (Hlookup & -> & ->)].
     apply step_store; auto.
+    eauto.
 Qed.
 
 Create HintDb step.
@@ -626,8 +640,8 @@ Proof.
 Qed.
 
 Lemma steps_alloc_val e m m' v l:
-  m' !! l = None →
-  steps e m (EVal v) m' → steps (EAlloc e) m (EVal (VLoc l)) (<[l:=v]> m').
+  valid_alloc m' l →
+  steps e m (EVal v) m' → steps (EAlloc e) m (EVal (VLoc l)) (<[l:=(Value v)]> m').
 Proof.
   intros U H.
   eapply steps_mono.
@@ -638,9 +652,9 @@ Proof.
   auto using steps_single with head_step.
 Qed.
 
-Lemma steps_free_val e m m' l:
-  m' !! l ≠ None →
-  steps e m (EVal (VLoc l)) m' → steps (EFree e) m (EVal VUnit) (delete l m').
+Lemma steps_free_val e m m' l v:
+   m' !! l = Some (Value v) →
+  steps e m (EVal (VLoc l)) m' → steps (EFree e) m (EVal VUnit) (<[ l := Reserved ]> m').
 Proof.
   intros U H.
   eapply steps_mono.
@@ -648,11 +662,11 @@ Proof.
   eapply steps_context.
   eassumption.
   rewrite fill_free.
-  auto using steps_single with head_step.
+  eauto using steps_single with head_step.
 Qed.
 
 Lemma steps_load_val e m m' l v:
-  m' !! l = Some(v) →
+  m' !! l = Some (Value v) →
   steps e m (EVal (VLoc l)) m' → steps (ELoad e) m (EVal v) m'.
 Proof.
   intros U H.
@@ -661,14 +675,14 @@ Proof.
   eapply steps_context.
   eassumption.
   rewrite fill_load.
-  auto using steps_single with head_step.
+  eauto using steps_single with head_step.
 Qed.
 
-Lemma steps_store_val e e' m m' m'' l v:
-  m'' !! l ≠ None →
+Lemma steps_store_val e e' m m' m'' l v w:
+  m'' !! l = Some (Value w) →
   steps e m (EVal (VLoc l)) m' →
   steps e' m' (EVal v) m'' →
-  steps (EStore e e') m (EVal VUnit) (<[l:=v]> m'').
+  steps (EStore e e') m (EVal VUnit) (<[l:= (Value v)]> m'').
 Proof.
   intros U Hl Hr.
   eapply steps_mono.
@@ -681,5 +695,5 @@ Proof.
   eapply steps_context.
   eassumption.
   rewrite fill_store_r.
-  auto using steps_single with head_step.
+  eauto using steps_single with head_step.
 Qed.
